Micro_C_Examples/Micro_C_Examples.thy
@@ -7,6 +7,7 @@ theory Micro_C_Examples
     C_Struct_Examples
     C_Array_Examples
     C_Bitwise_Examples
+    C_While_Examples
     "Micro_C_Interfaces.Micro_C_Interfaces"
 begin
 end
